{-# OPTIONS --without-K --rewriting #-}

module Omniscience where

open import Base
open import Base.WellFounded
open import Base.Equality
open import Base.Natural

open import Decreasing

LPO : Typeâ‚€
LPO = (f : â„• â†’ ğŸš) â†’ (Î£[ n âˆ¶ â„• ] f n â‰¡ 1â‚‚) âŠ (Î [ n âˆ¶ â„• ] f n â‰¡ 0â‚‚)

InfiniteValley : (â„• â†’ â„•) â†’ â„• â†’ Typeâ‚€
InfiniteValley f x = âˆ€ y â†’ x â‰¤ y â†’ f y â‰¡ f x

module LPOâ‡’InfiniteValleys where

  module _ (f : â„• â†’ â„•) where

    g : (â„• â†’ ğŸš)
    g x with f x â‰Ÿ f zero
    ... | iâ‚ _ = 0â‚‚
    ... | iâ‚‚ _ = 1â‚‚

    gâ‰¡0â‚‚-inv : âˆ€ {x} â†’ g x â‰¡ 0â‚‚ â†’ f x â‰¡ f zero
    gâ‰¡0â‚‚-inv {x} _ with f x â‰Ÿ f zero
    gâ‰¡0â‚‚-inv     _    | iâ‚ f[x]â‰¡f[0] = f[x]â‰¡f[0]
    gâ‰¡0â‚‚-inv     ()   | iâ‚‚ _

    gâ‰¡1â‚‚-Decreasing-inv : Decreasing f â†’ âˆ€ {x} â†’ g x â‰¡ 1â‚‚ â†’ f x < f zero
    gâ‰¡1â‚‚-Decreasing-inv dec {x} _ with f x â‰Ÿ f zero
    gâ‰¡1â‚‚-Decreasing-inv dec     ()   | iâ‚ _
    gâ‰¡1â‚‚-Decreasing-inv dec     _    | iâ‚‚ f[x]â‰¢f[0] = mâ‰¤nâ‡’mâ‰¢nâ‡’m<n (Decreasing-â‰¤ dec (0â‰¤n _)) f[x]â‰¢f[0]

  shift : âˆ€ {â„“} {A : Type â„“} â†’ â„• â†’ (â„• â†’ A) â†’ (â„• â†’ A)
  shift n f = Î» x â†’ f (x + n)

  shift-Decreasing : âˆ€ {f} â†’ Decreasing f â†’ âˆ€ n â†’ Decreasing (shift n f)
  shift-Decreasing dec n = Î» x â†’ dec (x + n)

  -- Let f : â„• â†’ â„• be decreasing. Use the limited principle of omniscience to
  -- determine whether gá¶  is 1â‚‚ somewhere or 0â‚‚ everywhere.
  -- 
  -- If gá¶  is 0â‚‚ everywhere, then f(x) = f(0) for all x by the inversion
  -- princple for g(x) = 0. This means that f has an infinite valley at 0.
  --
  -- If gá¶  is 1â‚‚ at x, recurse on shift x f. (We have shown above that this
  -- function is decreasing). The recursion will eventually terminate because
  -- f(x) < f(0) by the inversion principle for gá¶ (x) = 1â‚‚, and the less-than
  -- relationship is well-founded.
  --
  -- The recursive call yields y : â„• and v : InfiniteValley (shift x f) y. The
  -- expanded type of v is âˆ€ z â†’ y â‰¤ z â†’ f (z + x) â‰¡ f (y + x), so we take y + x
  -- as the starting point for the infinite valley in f.
  --
  -- Now we need to show that, for all z : â„•, if y + x â‰¤ z, then
  -- f(z) = f(y + x).
  --
  -- If y + x â‰¤ z, then z â‰¥ x. It follows that (z - x) + x = z, so
  -- f(z) = f((z - x) + x).
  --
  -- Again using the fact that y + x â‰¤ z, we conclude that y â‰¤ z - x. This means
  -- that z - x is in the valley v, so f((z - x) + x) = f(y + x). This concludes
  -- the proof.
  
  LPOâ‡’InfiniteValleys : LPO â†’ (f : â„• â†’ â„•) â†’ Decreasing f â†’ Î£ â„• (InfiniteValley f)
  LPOâ‡’InfiniteValleys lpo = Î» f dec â†’ WellFounded-induction (on-wf wf-< (Ï€â‚ â¨¾ _&_ 0)) _ go (f , dec) where

    _â‰º_ : Î£ (â„• â†’ â„•) Decreasing â†’ Î£ (â„• â†’ â„•) Decreasing â†’ Typeâ‚€
    (f , _) â‰º (g , _) = f zero < g zero

    go : âˆ€ u â†’ (âˆ€ w â†’ w â‰º u â†’ Î£ â„• (InfiniteValley (Ï€â‚ w))) â†’ Î£ â„• (InfiniteValley (Ï€â‚ u))
    go (f , dec) rec with lpo (g f)
    ... | iâ‚‚ gâ‰¡0â‚‚ = zero , (Î» x _ â†’ gâ‰¡0â‚‚-inv f (gâ‰¡0â‚‚ x))
    ... | iâ‚ (x , p) with rec (shift x f , shift-Decreasing dec x) (gâ‰¡1â‚‚-Decreasing-inv f dec p)
    ... | y , v = y + x , help where
      help : âˆ€ z â†’ y + x â‰¤ z â†’ f z â‰¡ f (y + x)
      help z y+xâ‰¤z = begin
        f z             â‰¡âŸ¨ mâ‰¤nâ‡’[n-m]+mâ‰¡n {x} (m+nâ‰¤pâ‡’nâ‰¤p {y} y+xâ‰¤z) |in-ctx f âŸ©â»Â¹
        f ((z - x) + x) â‰¡âŸ¨ v (z - x) (m+nâ‰¤pâ‡’mâ‰¤p-n y+xâ‰¤z) âŸ©
        f (y + x)       âˆ

module InfiniteValleysâ‡’LPO where

  -- An injection from ğŸš to â„•.

  i : ğŸš â†’ â„•
  i 0â‚‚ = 1
  i 1â‚‚ = 0

  -- Some basic facts about i.

  iâ‰¡0âŠiâ‰¡1 : âˆ€ x â†’ i x â‰¡ 0 âŠ i x â‰¡ 1
  iâ‰¡0âŠiâ‰¡1 0â‚‚ = iâ‚‚ refl
  iâ‰¡0âŠiâ‰¡1 1â‚‚ = iâ‚ refl

  iâ‰¤1 : âˆ€ x â†’ i x â‰¤ 1
  iâ‰¤1 x with i x | iâ‰¡0âŠiâ‰¡1 x
  ... | _ | iâ‚ refl = succ refl
  ... | _ | iâ‚‚ refl = refl

  iâ‰¡0-inv : âˆ€ {x} â†’ i x â‰¡ 0 â†’ x â‰¡ 1â‚‚
  iâ‰¡0-inv {0â‚‚} ()
  iâ‰¡0-inv {1â‚‚} _ = refl

  module _ (f : â„• â†’ ğŸš) where

    -- Intuitively, g(x) = 1 if f(y) = 0â‚‚ for all y â‰¤ x; otherwise, g(x) = 0.

    g : â„• â†’ â„•
    g zero = i (f zero)
    g (succ x) with g x
    ... | zero   = 0
    ... | succ _ = i (f (succ x))

    -- Either g(x) = 0 or g(x) = 1 for all x.

    gâ‰¡0âŠgâ‰¡1 : âˆ€ x â†’ g x â‰¡ 0 âŠ g x â‰¡ 1
    gâ‰¡0âŠgâ‰¡1 zero = iâ‰¡0âŠiâ‰¡1 (f zero)
    gâ‰¡0âŠgâ‰¡1 (succ x) with g x | gâ‰¡0âŠgâ‰¡1 x
    ... | _ | iâ‚ refl = iâ‚ refl
    ... | _ | iâ‚‚ refl = iâ‰¡0âŠiâ‰¡1 (f (succ x))

    -- Clearly, g is decreasing: g(x) â‰¤ 1 for all x; and if g(x) = 0, then
    -- g(y) = 0 for all y â‰¥ x.

    dec : Decreasing g
    dec zero with f 0
    ... | 1â‚‚ = refl
    ... | 0â‚‚ = iâ‰¤1 (f 1)
    dec (succ x) with g x | gâ‰¡0âŠgâ‰¡1 x
    ... | _ | iâ‚ refl = refl
    ... | _ | iâ‚‚ refl with f (succ x)
    ... | 0â‚‚ = iâ‰¤1 (f (succ (succ x)))
    ... | 1â‚‚ = refl

    -- If g(x) = 0, then there exists some y â‰¤ x such that f(y) = 1â‚‚.

    gâ‰¡0-inv : âˆ€ x â†’ g x â‰¡ 0 â†’ Î£[ y âˆ¶ â„• ] f y â‰¡ 1â‚‚
    gâ‰¡0-inv zero     i[f[0]]â‰¡0 = zero , iâ‰¡0-inv i[f[0]]â‰¡0
    gâ‰¡0-inv (succ x) i[f[sx]]â‰¡0 with g x | inspect g x | gâ‰¡0âŠgâ‰¡1 x
    ... | _ | [ g[x]â‰¡0 ] | iâ‚ refl = gâ‰¡0-inv x g[x]â‰¡0
    ... | _ | _          | iâ‚‚ refl = succ x , iâ‰¡0-inv i[f[sx]]â‰¡0

    -- If g(x) = 1, then f(x) = 0â‚‚.

    gâ‰¡1-inv : âˆ€ {x} â†’ g x â‰¡ 1 â†’ f x â‰¡ 0â‚‚
    gâ‰¡1-inv {zero}   _ with f zero
    gâ‰¡1-inv {zero}   _    | 0â‚‚ = refl
    gâ‰¡1-inv {zero}   ()   | 1â‚‚
    gâ‰¡1-inv {succ x} _ with g x | gâ‰¡0âŠgâ‰¡1 x
    gâ‰¡1-inv {succ x} ()   | _   | iâ‚ refl
    gâ‰¡1-inv {succ x} _    | _   | iâ‚‚ refl with f (succ x)
    gâ‰¡1-inv {succ x} _    | _   | iâ‚‚ refl    | 0â‚‚ = refl
    gâ‰¡1-inv {succ x} ()   | _   | iâ‚‚ refl    | 1â‚‚

    -- If g(x) = 1, then f(y) = 0â‚‚ for all y â‰¤ x.

    gâ‰¡1-inv-â‰¤ : âˆ€ {x} â†’ g x â‰¡ 1 â†’ âˆ€ {y} â†’ y â‰¤ x â†’ f y â‰¡ 0â‚‚
    gâ‰¡1-inv-â‰¤          g[x]â‰¡1 refl = gâ‰¡1-inv g[x]â‰¡1
    gâ‰¡1-inv-â‰¤ {succ x} _      (succ yâ‰¤x) with g x | inspect g x | gâ‰¡0âŠgâ‰¡1 x
    gâ‰¡1-inv-â‰¤ {succ x} ()     (succ yâ‰¤x)    | _   | _           | iâ‚ refl
    gâ‰¡1-inv-â‰¤ {succ x} _      (succ yâ‰¤x)    | _   | [ g[x]â‰¡1 ]  | iâ‚‚ refl = gâ‰¡1-inv-â‰¤ g[x]â‰¡1 yâ‰¤x

  -- Take f : ğŸš â†’ â„• and find a point x after which gá¶  remains constant.
  --
  -- If gá¶ (x) = 0, then there exists some y â‰¤ x such that f(y) = 1â‚‚, as shown
  -- above. (In this case it does not even matter that gá¶  remains constant.)
  --
  -- If gá¶ (x) = 1, then f is 0â‚‚ everywhere by the following argument:
  --
  -- Take y : â„•. Determine whether y â‰¤ x (this can be done constructively).
  --
  -- If y â‰¤ x, then f(y) = 0â‚‚ by the generalized inversion principle for
  -- g(x) = 1.
  --
  -- If y â‰° x, then y â‰¥ x. Since gá¶  is constant after x, gá¶ (y) = 1, so
  -- f(y) = 0â‚‚.

  InfiniteValleysâ‡’LPO : (âˆ€ f â†’ Decreasing f â†’ Î£ â„• (InfiniteValley f)) â†’ LPO
  InfiniteValleysâ‡’LPO vs f with vs (g f) (dec f)
  ... | x , v with g f x | inspect (g f) x | gâ‰¡0âŠgâ‰¡1 f x
  ... | _ | [ g[x]â‰¡0 ] | iâ‚ refl = iâ‚ (gâ‰¡0-inv f x g[x]â‰¡0)
  ... | _ | [ g[x]â‰¡1 ] | iâ‚‚ refl = iâ‚‚ (Î» y â†’ case y â‰¤? x of Î»{ (iâ‚ yâ‰¤x) â†’ gâ‰¡1-inv-â‰¤ f g[x]â‰¡1 yâ‰¤x
                                                             ; (iâ‚‚ yâ‰°x) â†’ gâ‰¡1-inv f (v y (â‰°â‡’â‰¥ yâ‰°x))
                                                             })
